Datalog/Bit_Vector_Framework.thy
@@ -41,56 +41,34 @@ datatype ('n,'a,'d) cst =
   | is_Elem: Elem (the_Elem: 'd)
   | is_Action: Action (the_Action: "'a")
 
-abbreviation may_Cls 
-  :: "(var, ('n,'v,'d) cst) id list \<Rightarrow> 
-      (pred, var, ('n,'v,'d) cst) rh list \<Rightarrow> 
-      (pred, var, ('n,'v,'d) cst) clause" ("may\<langle>_\<rangle> :- _ .") where
+abbreviation may_Cls :: "(var, ('n,'v,'d) cst) id list \<Rightarrow> (pred, var, ('n,'v,'d) cst) rh list \<Rightarrow> (pred, var, ('n,'v,'d) cst) clause" ("may\<langle>_\<rangle> :- _ .") where 
    "may\<langle>ids\<rangle> :- ls. \<equiv> Cls the_may ids ls"
 
-abbreviation must_Cls 
-  :: "(var, ('n,'v,'d) cst) id list \<Rightarrow> 
-      (pred, var, ('n,'v,'d) cst) rh list \<Rightarrow> 
-      (pred, var, ('n,'v,'d) cst) clause" ("must\<langle>_\<rangle> :- _ .") where
+abbreviation must_Cls :: "(var, ('n,'v,'d) cst) id list \<Rightarrow> (pred, var, ('n,'v,'d) cst) rh list \<Rightarrow> (pred, var, ('n,'v,'d) cst) clause" ("must\<langle>_\<rangle> :- _ .") where
   "must\<langle>ids\<rangle> :- ls. \<equiv> Cls the_must ids ls"
 
-abbreviation init_Cls 
-  :: "(var, ('n,'v,'d) cst) id list \<Rightarrow> 
-      (pred, var, ('n,'v,'d) cst) rh list \<Rightarrow> 
-      (pred, var, ('n,'v,'d) cst) clause" ("init\<langle>_\<rangle> :- _ .") where 
+abbreviation init_Cls :: "(var, ('n,'v,'d) cst) id list \<Rightarrow> (pred, var, ('n,'v,'d) cst) rh list \<Rightarrow> (pred, var, ('n,'v,'d) cst) clause" ("init\<langle>_\<rangle> :- _ .") where 
   "init\<langle>ids\<rangle> :- ls. \<equiv> Cls the_init ids ls"
 
-abbreviation anadom_Cls 
-  :: "(var, ('n,'v,'d) cst) id list \<Rightarrow> 
-      (pred, var, ('n,'v,'d) cst) rh list \<Rightarrow> 
-      (pred, var, ('n,'v,'d) cst) clause" ("anadom\<langle>_\<rangle> :- _ .") where 
+abbreviation anadom_Cls :: "(var, ('n,'v,'d) cst) id list \<Rightarrow> (pred, var, ('n,'v,'d) cst) rh list \<Rightarrow> (pred, var, ('n,'v,'d) cst) clause" ("anadom\<langle>_\<rangle> :- _ .") where 
   "anadom\<langle>ids\<rangle> :- ls. \<equiv> Cls the_anadom ids ls"
 
-abbreviation kill_Cls 
-  :: "(var, ('n,'v,'d) cst) id list \<Rightarrow> 
-      (pred, var, ('n,'v,'d) cst) rh list \<Rightarrow> 
-      (pred, var, ('n,'v,'d) cst) clause" ("kill\<langle>_\<rangle> :- _ .") where 
+abbreviation kill_Cls :: "(var, ('n,'v,'d) cst) id list \<Rightarrow> (pred, var, ('n,'v,'d) cst) rh list \<Rightarrow> (pred, var, ('n,'v,'d) cst) clause" ("kill\<langle>_\<rangle> :- _ .") where 
   "kill\<langle>ids\<rangle> :- ls. \<equiv> Cls the_kill ids ls"
 
-abbreviation gen_Cls 
-  :: "(var, ('n,'v,'d) cst) id list \<Rightarrow> 
-      (pred, var, ('n,'v,'d) cst) rh list \<Rightarrow> 
-      (pred, var, ('n,'v,'d) cst) clause" ("gen\<langle>_\<rangle> :- _ .") where 
+abbreviation gen_Cls :: "(var, ('n,'v,'d) cst) id list \<Rightarrow> (pred, var, ('n,'v,'d) cst) rh list \<Rightarrow> (pred, var, ('n,'v,'d) cst) clause" ("gen\<langle>_\<rangle> :- _ .") where 
   "gen\<langle>ids\<rangle> :- ls. \<equiv> Cls the_gen ids ls"
 
-abbreviation BV_lh :: "(var, ('n,'v,'d) cst) id list \<Rightarrow> (pred, var, ('n,'v,'d) cst) lh" 
-  ("may\<langle>_\<rangle>.") where  
+abbreviation BV_lh :: "(var, ('n,'v,'d) cst) id list \<Rightarrow> (pred, var, ('n,'v,'d) cst) lh" ("may\<langle>_\<rangle>.") where  
   "may\<langle>ids\<rangle>. \<equiv> (the_may, ids)"
 
-abbreviation must_lh :: "(var, ('n,'v,'d) cst) id list \<Rightarrow> (pred, var, ('n,'v,'d) cst) lh" 
-  ("must\<langle>_\<rangle>.") where 
+abbreviation must_lh :: "(var, ('n,'v,'d) cst) id list \<Rightarrow> (pred, var, ('n,'v,'d) cst) lh" ("must\<langle>_\<rangle>.") where 
   "must\<langle>ids\<rangle>. \<equiv> (the_must, ids)"
 
-abbreviation init_lh :: "(var, ('n,'v,'d) cst) id list \<Rightarrow> (pred, var, ('n,'v,'d) cst) lh" 
-  ("init\<langle>_\<rangle>.") where
+abbreviation init_lh :: "(var, ('n,'v,'d) cst) id list \<Rightarrow> (pred, var, ('n,'v,'d) cst) lh" ("init\<langle>_\<rangle>.") where
   "init\<langle>ids\<rangle>. \<equiv> (the_init, ids)"
 
-abbreviation dom_lh :: "(var, ('n,'v,'d) cst) id list \<Rightarrow> (pred, var, ('n,'v,'d) cst) lh" 
-  ("anadom\<langle>_\<rangle>.") where
+abbreviation dom_lh :: "(var, ('n,'v,'d) cst) id list \<Rightarrow> (pred, var, ('n,'v,'d) cst) lh" ("anadom\<langle>_\<rangle>.") where
   "anadom\<langle>ids\<rangle>. \<equiv> (the_anadom, ids)"
 
 abbreviation \<uu> :: "(var, 'a) id" where
@@ -139,8 +117,7 @@ locale analysis_BV_forward_may = finite_program_graph pg
 begin
 
 lemma finite_d_init: "finite d_init"
-  by (meson analysis_BV_forward_may_axioms analysis_BV_forward_may_axioms_def 
-      analysis_BV_forward_may_def rev_finite_subset)
+  by (meson analysis_BV_forward_may_axioms analysis_BV_forward_may_axioms_def analysis_BV_forward_may_def rev_finite_subset)
 
 interpretation LTS edges .
 
@@ -200,8 +177,7 @@ definition ana_kill_edge :: "('n, 'a) edge \<Rightarrow> (pred, var, ('n, 'a, 'd
   "ana_kill_edge e = ana_kill_edge_d e ` (kill_set e)"
 
 lemma kill_set_eq_kill_set_inter_analysis_dom: "kill_set e = kill_set e \<inter> analysis_dom"
-  by (meson analysis_BV_forward_may_axioms analysis_BV_forward_may_axioms_def 
-      analysis_BV_forward_may_def inf.orderE)
+  by (meson analysis_BV_forward_may_axioms analysis_BV_forward_may_axioms_def analysis_BV_forward_may_def inf.orderE)
 
 fun ana_gen_edge_d :: "('n, 'a) edge \<Rightarrow> 'd \<Rightarrow> (pred, var, ('n, 'a, 'd) cst) clause" where
   "ana_gen_edge_d (q\<^sub>o, \<alpha>, q\<^sub>s) d = gen\<langle>[Cst\<^sub>N q\<^sub>o, Cst\<^sub>A \<alpha>, Cst\<^sub>N q\<^sub>s, Cst\<^sub>E d]\<rangle> :- []."
@@ -210,8 +186,7 @@ definition ana_gen_edge :: "('n, 'a) edge \<Rightarrow> (pred, var, ('n, 'a, 'd)
   "ana_gen_edge e = ana_gen_edge_d e ` (gen_set e)"
 
 lemma gen_set_eq_gen_set_inter_analysis_dom: "gen_set e = gen_set e \<inter> analysis_dom"
-  by (meson analysis_BV_forward_may_axioms analysis_BV_forward_may_axioms_def 
-      analysis_BV_forward_may_def inf.orderE)
+  by (meson analysis_BV_forward_may_axioms analysis_BV_forward_may_axioms_def analysis_BV_forward_may_def inf.orderE)
 
 definition ana_init :: "'d \<Rightarrow> (pred, var, ('n, 'a, 'd) cst) clause" where
   "ana_init d = init\<langle>[Cst\<^sub>E d]\<rangle> :- []."
@@ -278,8 +253,7 @@ lemma S_hat_path_append:
   shows "S^\<^sub>P\<lbrakk>(qs @ [qnminus1, qn], w @ [\<alpha>])\<rbrakk> d_init =
     S^\<^sub>E\<lbrakk>(qnminus1, \<alpha>, qn)\<rbrakk> (S^\<^sub>P\<lbrakk>(qs @ [qnminus1], w)\<rbrakk> d_init)"
 proof -
-  have "S^\<^sub>P\<lbrakk> (qs @ [qnminus1, qn], w @ [\<alpha>])\<rbrakk> d_init = 
-        S^\<^sub>E\<^sub>s\<lbrakk>(transition_list (qs @ [qnminus1, qn], w @ [\<alpha>]))\<rbrakk> d_init"
+  have "S^\<^sub>P\<lbrakk> (qs @ [qnminus1, qn], w @ [\<alpha>])\<rbrakk> d_init = S^\<^sub>E\<^sub>s\<lbrakk>(transition_list (qs @ [qnminus1, qn], w @ [\<alpha>]))\<rbrakk> d_init"
     unfolding S_hat_path_def by auto
   moreover
   have "S^\<^sub>E\<^sub>s\<lbrakk>(transition_list (qs @ [qnminus1, qn], w @ [\<alpha>]))\<rbrakk> d_init =
@@ -287,9 +261,8 @@ proof -
     using transition_list_reversed_simp[of qs w] assms
     by auto
   moreover
-  have 
-    "... = S^\<^sub>E\<^sub>s\<lbrakk>[(qnminus1, \<alpha>, qn)]\<rbrakk> (S_hat_edge_list (transition_list (qs @ [qnminus1], w)) d_init)"
-    using S_hat_edge_list_append[of "transition_list (qs @ [qnminus1], w)" "[(qnminus1, \<alpha>, qn)]" d_init]
+  have "... = S^\<^sub>E\<^sub>s\<lbrakk>[(qnminus1, \<alpha>, qn)]\<rbrakk> (S_hat_edge_list (transition_list (qs @ [qnminus1], w)) d_init)"
+    using S_hat_edge_list_append[of "transition_list (qs @ [qnminus1], w)" " [(qnminus1, \<alpha>, qn)]" d_init]
     by auto
   moreover
   have "... = S^\<^sub>E\<lbrakk>(qnminus1, \<alpha>, qn)\<rbrakk> (S^\<^sub>P\<lbrakk> (qs @ [qnminus1], w)\<rbrakk> d_init)"
@@ -387,19 +360,17 @@ proof -
     using lh_consequence_def by metis
   ultimately
   show "\<rho> \<Turnstile>\<^sub>r\<^sub>h \<^bold>\<not>kill [Cst\<^sub>N q\<^sub>o, Cst\<^sub>A \<alpha>, Cst\<^sub>N q\<^sub>s, Cst\<^sub>E d]"
-    using solves_NegLit_least[of ana_pg_fw_may \<rho> s_BV "[Cst\<^sub>N q\<^sub>o, Cst\<^sub>A \<alpha>, Cst\<^sub>N q\<^sub>s, Cst\<^sub>E d]" the_kill] 
-    by auto
+    using solves_NegLit_least[of ana_pg_fw_may \<rho> s_BV "[Cst\<^sub>N q\<^sub>o, Cst\<^sub>A \<alpha>, Cst\<^sub>N q\<^sub>s, Cst\<^sub>E d]" the_kill] by auto
 qed
 
 lemma S_hat_edge_list_subset_analysis_dom:
-  assumes "d \<in> S^\<^sub>E\<^sub>s\<lbrakk>\<pi>\<rbrakk> d_init"
-  shows "d \<in> analysis_dom"
-  using assms
+  "d \<in> S^\<^sub>E\<^sub>s\<lbrakk>\<pi>\<rbrakk> d_init \<Longrightarrow> d \<in> analysis_dom"
 proof(induction \<pi> rule: List.rev_induct)
   case Nil
   then show ?case
     by (metis S_hat_edge_list.simps(1) analysis_BV_forward_may.axioms(2) 
         analysis_BV_forward_may_axioms analysis_BV_forward_may_axioms_def subsetD)
+
 next
   case (snoc e \<pi>)
   have "gen_set e \<inter> analysis_dom \<subseteq> analysis_dom"
@@ -409,14 +380,12 @@ next
 qed
 
 lemma S_hat_path_subset_analysis_dom:
-  assumes "d \<in> S^\<^sub>P\<lbrakk>(ss,w)\<rbrakk> d_init"
-  shows "d \<in> analysis_dom"
-  using assms S_hat_path_def S_hat_edge_list_subset_analysis_dom by auto
+  "d \<in> S^\<^sub>P\<lbrakk>(ss,w)\<rbrakk> d_init \<Longrightarrow> d \<in> analysis_dom"
+  using S_hat_path_def S_hat_edge_list_subset_analysis_dom by auto
 
 lemma S_hat_path_last:
   assumes "length qs = length w"
-  shows "S^\<^sub>P\<lbrakk>(qs @ [qnminus1, qn], w @ [\<alpha>])\<rbrakk> d_init =
-         S^\<^sub>E\<lbrakk>(qnminus1, \<alpha>, qn)\<rbrakk> (S^\<^sub>P\<lbrakk>(qs @ [qnminus1], w)\<rbrakk> d_init)"
+  shows "S^\<^sub>P\<lbrakk>(qs @ [qnminus1, qn], w @ [\<alpha>])\<rbrakk> d_init = S^\<^sub>E\<lbrakk>(qnminus1, \<alpha>, qn)\<rbrakk> (S^\<^sub>P\<lbrakk>(qs @ [qnminus1], w)\<rbrakk> d_init)"
   using assms transition_list_reversed_simp unfolding S_hat_path_def by force
 
 lemma gen_sound:
@@ -469,8 +438,7 @@ next
   
   have "d \<in> S^\<^sub>E\<lbrakk>(qnminus1, \<alpha>, qn)\<rbrakk> (S^\<^sub>P\<lbrakk>(qs @ [qnminus1], w)\<rbrakk> d_init)"
     using "2.prems"(2) S_hat_path_last len by blast
-  then have "d \<in> (S^\<^sub>P\<lbrakk>(qs @ [qnminus1], w)\<rbrakk> d_init) - kill_set (qnminus1, \<alpha>, qn) \<or>
-             d \<in> gen_set (qnminus1, \<alpha>, qn)"
+  then have "d \<in> (S^\<^sub>P\<lbrakk>(qs @ [qnminus1], w)\<rbrakk> d_init) - kill_set (qnminus1, \<alpha>, qn) \<or> d \<in> gen_set (qnminus1, \<alpha>, qn)"
     unfolding S_hat_def by simp
   then show ?case
   proof 
@@ -481,25 +449,20 @@ next
     from dSnotkill have "\<rho> \<Turnstile>\<^sub>r\<^sub>h \<^bold>\<not>kill [Cst\<^sub>N qnminus1, Cst\<^sub>A \<alpha>, Cst\<^sub>N qn, Cst\<^sub>E d]"
       using not_kill[of d qnminus1 \<alpha> qn \<rho>] 2(6) by auto
     moreover
-    have "\<rho> \<Turnstile>\<^sub>c\<^sub>l\<^sub>s may\<langle>[Cst\<^sub>N qn, \<uu>]\<rangle> :- [may [Cst\<^sub>N qnminus1, \<uu>],
-                                      \<^bold>\<not>kill [Cst\<^sub>N qnminus1, Cst\<^sub>A \<alpha>, Cst\<^sub>N qn, \<uu>]]."
-      using 2(6) "2.hyps"(2) 
-      by (force simp add: ana_pg_fw_may_def solves_program_def least_solution_def)
-    then have "\<rho> \<Turnstile>\<^sub>c\<^sub>l\<^sub>s may\<langle>[Cst\<^sub>N qn, Cst\<^sub>E d]\<rangle> :- [may [Cst\<^sub>N qnminus1, Cst\<^sub>E d], 
-                                               \<^bold>\<not>kill [Cst\<^sub>N qnminus1, Cst\<^sub>A \<alpha>, Cst\<^sub>N qn, Cst\<^sub>E d]]."
+    have "\<rho> \<Turnstile>\<^sub>c\<^sub>l\<^sub>s may\<langle>[Cst\<^sub>N qn, \<uu>]\<rangle> :- [may [Cst\<^sub>N qnminus1, \<uu>], \<^bold>\<not>kill [Cst\<^sub>N qnminus1, Cst\<^sub>A \<alpha>, Cst\<^sub>N qn, \<uu>]] ."
+      using 2(6) "2.hyps"(2) by (force simp add: ana_pg_fw_may_def solves_program_def least_solution_def)
+    then have "\<rho> \<Turnstile>\<^sub>c\<^sub>l\<^sub>s may\<langle>[Cst\<^sub>N qn, Cst\<^sub>E d]\<rangle> :- [may [Cst\<^sub>N qnminus1, Cst\<^sub>E d], \<^bold>\<not>kill [Cst\<^sub>N qnminus1, Cst\<^sub>A \<alpha>, Cst\<^sub>N qn, Cst\<^sub>E d]]."
       using substitution_lemma[of \<rho> _ "\<lambda>u. Cst\<^sub>E d"] by force
     ultimately 
     have "\<rho> \<Turnstile>\<^sub>l\<^sub>h may\<langle>[Cst\<^sub>N qn, Cst\<^sub>E d]\<rangle>."
-      by (metis (no_types, lifting) Cons_eq_appendI prop_inf_last_from_cls_rh_to_cls modus_ponens_rh 
-          self_append_conv2)
+      by (metis (no_types, lifting) Cons_eq_appendI prop_inf_last_from_cls_rh_to_cls modus_ponens_rh self_append_conv2)
     then show "?case"
       by (auto simp add: LTS.end_of_def)
   next
     assume d_gen: "d \<in> gen_set (qnminus1, \<alpha>, qn)"
 
     have "\<forall>c\<in>ana_edge (qnminus1, \<alpha>, qn). \<rho> \<Turnstile>\<^sub>c\<^sub>l\<^sub>s c"
-      using 2(6) "2.hyps"(2) unfolding ana_pg_fw_may_def solves_program_def least_solution_def 
-      by blast
+      using 2(6) "2.hyps"(2) unfolding ana_pg_fw_may_def solves_program_def least_solution_def by blast
     then have "\<rho> \<Turnstile>\<^sub>c\<^sub>l\<^sub>s may\<langle>[Cst\<^sub>N qn, \<uu>]\<rangle> :- [gen [Cst\<^sub>N qnminus1, Cst\<^sub>A \<alpha>, Cst\<^sub>N qn, \<uu>]] ."
       by auto
     then have "\<rho> \<Turnstile>\<^sub>c\<^sub>l\<^sub>s may\<langle>[Cst\<^sub>N qn, Cst\<^sub>E d]\<rangle> :- [gen [Cst\<^sub>N qnminus1, Cst\<^sub>A \<alpha>, Cst\<^sub>N qn, Cst\<^sub>E d]] ."
@@ -588,9 +551,8 @@ definition S_hat_path :: "('n list \<times> 'a list) \<Rightarrow> 'd set \<Righ
   "S^\<^sub>P\<lbrakk>\<pi>\<rbrakk> R = S^\<^sub>E\<^sub>s\<lbrakk>(transition_list \<pi>)\<rbrakk> R"
 
 definition summarizes_bw_may :: "(pred, ('n, 'a, 'd) cst) pred_val \<Rightarrow> bool" where
-  "summarizes_bw_may \<rho> \<longleftrightarrow> (\<forall>\<pi> d. \<pi> \<in> path_with_word_to end \<longrightarrow> 
-                                  d \<in> S^\<^sub>P\<lbrakk>\<pi>\<rbrakk> d_init \<longrightarrow> 
-                                  \<rho> \<Turnstile>\<^sub>l\<^sub>h may\<langle>[Cst\<^sub>N (start_of \<pi>), Cst\<^sub>E d]\<rangle>.)"
+  "summarizes_bw_may \<rho> \<longleftrightarrow> (\<forall>\<pi> d. \<pi> \<in> path_with_word_to end \<longrightarrow> d \<in> S^\<^sub>P\<lbrakk>\<pi>\<rbrakk> d_init \<longrightarrow> 
+                             \<rho> \<Turnstile>\<^sub>l\<^sub>h may\<langle>[Cst\<^sub>N (start_of \<pi>), Cst\<^sub>E d]\<rangle>.)"
 
 lemma kill_subs_analysis_dom: "(kill_set (rev_edge e)) \<subseteq> analysis_dom"
   by (meson analysis_BV_backward_may_axioms analysis_BV_backward_may_axioms_def 
@@ -600,10 +562,8 @@ lemma gen_subs_analysis_dom: "(gen_set (rev_edge e)) \<subseteq> analysis_dom"
   by (meson analysis_BV_backward_may.axioms(2) analysis_BV_backward_may_axioms 
       analysis_BV_backward_may_axioms_def)
 
-interpretation fw_may: analysis_BV_forward_may 
-  pg_rev analysis_dom "\<lambda>e. (kill_set (rev_edge e))" "(\<lambda>e. gen_set (rev_edge e))" d_init
-  using analysis_BV_forward_may_def finite_pg_rev analysis_BV_backward_may_axioms 
-    analysis_BV_backward_may_def
+interpretation fw_may: analysis_BV_forward_may pg_rev analysis_dom "\<lambda>e. (kill_set (rev_edge e))" "(\<lambda>e. gen_set (rev_edge e))" d_init
+  using analysis_BV_forward_may_def finite_pg_rev analysis_BV_backward_may_axioms analysis_BV_backward_may_def
   by (metis (no_types, lifting) analysis_BV_backward_may_axioms_def 
       analysis_BV_forward_may_axioms_def finite_program_graph_def program_graph.edges_def)
  
@@ -764,14 +724,9 @@ definition summarizes_fw_must :: "(pred, ('n, 'a, 'd) cst) pred_val \<Rightarrow
    "summarizes_fw_must \<rho> \<longleftrightarrow>
      (\<forall>q d.
          \<rho> \<Turnstile>\<^sub>l\<^sub>h must\<langle>[q, d]\<rangle>. \<longrightarrow>
-           (\<forall>\<pi>. \<pi> \<in> path_with_word \<longrightarrow>
-                start_of \<pi> = start \<longrightarrow>
-                end_of \<pi> = the_Node\<^sub>i\<^sub>d q \<longrightarrow>
-                (the_Elem\<^sub>i\<^sub>d d) \<in> S^\<^sub>P\<lbrakk>\<pi>\<rbrakk> d_init))"
+          (\<forall>\<pi>. \<pi> \<in> path_with_word \<longrightarrow> start_of \<pi> = start \<longrightarrow> end_of \<pi> = the_Node\<^sub>i\<^sub>d q \<longrightarrow> (the_Elem\<^sub>i\<^sub>d d) \<in> S^\<^sub>P\<lbrakk>\<pi>\<rbrakk> d_init))"
 
-interpretation fw_may: analysis_BV_forward_may 
-  pg analysis_dom "\<lambda>e. analysis_dom - (kill_set e)" "(\<lambda>e. analysis_dom - gen_set e)" 
-  "analysis_dom - d_init"
+interpretation fw_may: analysis_BV_forward_may pg analysis_dom "\<lambda>e. analysis_dom - (kill_set e)" "(\<lambda>e. analysis_dom - gen_set e)" "analysis_dom - d_init"
   using analysis_BV_forward_may.intro[of pg] analysis_BV_forward_must_def[of pg] 
     analysis_BV_forward_may_axioms_def analysis_BV_forward_must_axioms 
     analysis_BV_forward_must_axioms_def by (metis Diff_subset)
@@ -931,13 +886,13 @@ lemma is_Cst_if_init:
   shows "is_Cst d"
 proof (rule ccontr)
   assume "\<not> is_Cst d"
-  then have du: "d = \<uu>"
+  then have qu: "d = \<uu>"
     by (metis (full_types) id.disc(1) id.exhaust_disc id.expand var.exhaust)
   then have "\<lbrakk>init\<langle>[d]\<rangle>.\<rbrakk>\<^sub>l\<^sub>h \<rho> (\<lambda>x. Action undefined)" 
     using assms
     by auto
   then have "\<rho> \<Turnstile>\<^sub>l\<^sub>h init\<langle>[d \<cdot>\<^sub>v\<^sub>i\<^sub>d (\<lambda>x. Action undefined)]\<rangle>."
-    using solves_lh_substv_lh_if_meaning_lh[of "init\<langle>[d]\<rangle>." \<rho> "(\<lambda>x. Action undefined)"] du by auto
+    using solves_lh_substv_lh_if_meaning_lh[of "init\<langle>[d]\<rangle>." \<rho> "(\<lambda>x. Action undefined)"] qu by auto
   moreover
   have "is_Cst (Cst\<^sub>A undefined)"
     by auto
@@ -946,7 +901,7 @@ proof (rule ccontr)
     by (metis id.disc(4) substv_id.elims)
   ultimately
   have "\<exists>c \<in> ana_pg_fw_must. lh_consequence \<rho> c (init\<langle>[Cst\<^sub>A undefined]\<rangle>.)"
-    using solves_lh_least[of ana_pg_fw_must \<rho> s_BV] du
+    using solves_lh_least[of ana_pg_fw_must \<rho> s_BV] qu
     by (simp add: assms(1) fw_may.ana_pg_fw_may_finite fw_may.ana_pg_fw_may_stratified)
   then show False
     unfolding fw_may.ana_pg_fw_may_def fw_may.ana_entry_node_def lh_consequence_def
@@ -960,13 +915,13 @@ lemma is_Cst_if_anadom:
   shows "is_Cst d"
 proof (rule ccontr)
   assume "\<not> is_Cst d"
-  then have du: "d = \<uu>"
+  then have qu: "d = \<uu>"
     by (metis (full_types) id.disc(1) id.exhaust_disc id.expand var.exhaust)
   then have "\<lbrakk>anadom\<langle>[d]\<rangle>.\<rbrakk>\<^sub>l\<^sub>h \<rho> (\<lambda>x. Action undefined)" 
     using assms
     by auto
   then have "\<rho> \<Turnstile>\<^sub>l\<^sub>h anadom\<langle>[d \<cdot>\<^sub>v\<^sub>i\<^sub>d (\<lambda>x. Action undefined)]\<rangle>."
-    using solves_lh_substv_lh_if_meaning_lh[of "anadom\<langle>[d]\<rangle>." \<rho> "(\<lambda>x. Action undefined)"] du by auto
+    using solves_lh_substv_lh_if_meaning_lh[of "anadom\<langle>[d]\<rangle>." \<rho> "(\<lambda>x. Action undefined)"] qu by auto
   moreover
   have "is_Cst (Cst\<^sub>A undefined)"
     by auto
@@ -975,7 +930,7 @@ proof (rule ccontr)
     by (metis id.disc(4) substv_id.elims)
   ultimately
   have "\<exists>c \<in> ana_pg_fw_must. lh_consequence \<rho> c (anadom\<langle>[Cst\<^sub>A undefined]\<rangle>.)"
-    using solves_lh_least[of ana_pg_fw_must \<rho> s_BV] du
+    using solves_lh_least[of ana_pg_fw_must \<rho> s_BV] qu
     by (simp add: assms(1) fw_may.ana_pg_fw_may_finite fw_may.ana_pg_fw_may_stratified)
   then show False
     unfolding fw_may.ana_pg_fw_may_def fw_may.ana_entry_node_def lh_consequence_def
@@ -988,10 +943,10 @@ lemma if_init:
   assumes "\<rho> \<Turnstile>\<^sub>l\<^sub>h init\<langle>[d]\<rangle>."
   shows "is_Elem\<^sub>i\<^sub>d d \<and> the_Elem\<^sub>i\<^sub>d d \<in> (analysis_dom - d_init)"
 proof -
-  have d_Cst: "is_Cst d"
+  have Csts: "is_Cst d"
     using assms(1) assms(2) is_Cst_if_init by blast
 
-  from assms(1,2) d_Cst have "\<exists>c \<in> ana_pg_fw_must. lh_consequence \<rho> c (init\<langle>[d]\<rangle>.)"
+  from assms(1,2) Csts have "\<exists>c \<in> ana_pg_fw_must. lh_consequence \<rho> c (init\<langle>[d]\<rangle>.)"
     using solves_lh_least[of ana_pg_fw_must \<rho> s_BV "[d]"] fw_may.ana_pg_fw_may_finite
       fw_may.ana_pg_fw_may_stratified by fastforce
 
@@ -1026,10 +981,10 @@ lemma if_anadom:
   assumes "\<rho> \<Turnstile>\<^sub>l\<^sub>h anadom\<langle>[d]\<rangle>."
   shows "is_Elem\<^sub>i\<^sub>d d \<and> the_Elem\<^sub>i\<^sub>d d \<in> analysis_dom"
 proof -
-  have d_Cst: "is_Cst d"
+  have Csts: "is_Cst d"
     using assms(1) assms(2) is_Cst_if_anadom by blast
 
-  from assms(1,2) d_Cst have "\<exists>c \<in> ana_pg_fw_must. lh_consequence \<rho> c (anadom\<langle>[d]\<rangle>.)"
+  from assms(1,2) Csts have "\<exists>c \<in> ana_pg_fw_must. lh_consequence \<rho> c (anadom\<langle>[d]\<rangle>.)"
     using solves_lh_least[of ana_pg_fw_must \<rho> s_BV "[d]"] fw_may.ana_pg_fw_may_finite
       fw_may.ana_pg_fw_may_stratified by fastforce
   then obtain c where 
@@ -1144,13 +1099,13 @@ lemma must_snd_id_is_Cst:
   shows "is_Cst d"
 proof (rule ccontr)
   assume "\<not> is_Cst d"
-  then have du: "d = \<uu>"
+  then have qu: "d = \<uu>"
     by (metis (full_types) id.disc(1) id.exhaust_disc id.expand var.exhaust)
   then have "\<lbrakk>must\<langle>[q,d]\<rangle>.\<rbrakk>\<^sub>l\<^sub>h \<rho> (\<lambda>x. Action undefined)" 
     using assms
     by auto
   then have "\<rho> \<Turnstile>\<^sub>l\<^sub>h must\<langle>[q \<cdot>\<^sub>v\<^sub>i\<^sub>d (\<lambda>x. Action undefined), Cst\<^sub>A undefined]\<rangle>."
-    using solves_lh_substv_lh_if_meaning_lh[of "must\<langle>[q, d]\<rangle>." \<rho> "(\<lambda>x. Action undefined)"] du by auto
+    using solves_lh_substv_lh_if_meaning_lh[of "must\<langle>[q, d]\<rangle>." \<rho> "(\<lambda>x. Action undefined)"] qu by auto
   moreover
   have "is_Cst (Cst\<^sub>A undefined)"
     by auto
@@ -1172,11 +1127,10 @@ proof (rule ccontr)
       fw_may.ana_must_def by auto
   then obtain q' where "c = must\<langle>[Cst\<^sub>N q',\<uu>]\<rangle> :- [\<^bold>\<not>may[Cst\<^sub>N q',\<uu>], anadom[\<uu>]]."
     by auto
-  then have "lh_consequence \<rho> (must\<langle>[Cst\<^sub>N q',\<uu>]\<rangle> :- [\<^bold>\<not>may[Cst\<^sub>N q',\<uu>], anadom[\<uu>]].) 
-                              (must\<langle>[q \<cdot>\<^sub>v\<^sub>i\<^sub>d (\<lambda>x. Action undefined), Cst\<^sub>A undefined]\<rangle>.)"
+  then have "lh_consequence \<rho> (must\<langle>[Cst\<^sub>N q',\<uu>]\<rangle> :- [\<^bold>\<not>may[Cst\<^sub>N q',\<uu>], anadom[\<uu>]].) (must\<langle>[q \<cdot>\<^sub>v\<^sub>i\<^sub>d (\<lambda>x. Action undefined), Cst\<^sub>A undefined]\<rangle>.)"
     using c_p(2) by auto
-  then have "\<exists>\<sigma>'. (must\<langle>[Cst\<^sub>N q', \<uu>]\<rangle>. \<cdot>\<^sub>v\<^sub>l\<^sub>h \<sigma>') = must\<langle>[q \<cdot>\<^sub>v\<^sub>i\<^sub>d (\<lambda>x. Action undefined), Cst\<^sub>A undefined]\<rangle>.
-                  \<and> \<lbrakk>[\<^bold>\<not>may[Cst\<^sub>N q', \<uu>], anadom[\<uu>]]\<rbrakk>\<^sub>r\<^sub>h\<^sub>s \<rho> \<sigma>'"
+  then have "\<exists>\<sigma>'. (must\<langle>[Cst\<^sub>N q', \<uu>]\<rangle>. \<cdot>\<^sub>v\<^sub>l\<^sub>h \<sigma>') = must\<langle>[q \<cdot>\<^sub>v\<^sub>i\<^sub>d (\<lambda>x. Action undefined), Cst\<^sub>A undefined]\<rangle>. \<and>
+        \<lbrakk>[\<^bold>\<not>may[Cst\<^sub>N q', \<uu>], anadom[\<uu>]]\<rbrakk>\<^sub>r\<^sub>h\<^sub>s \<rho> \<sigma>'"
     unfolding lh_consequence_def using the_lh.simps clause.sel(3) by metis
   then obtain \<sigma>' where \<sigma>'_p:
     "(must\<langle>[Cst\<^sub>N q', \<uu>]\<rangle>. \<cdot>\<^sub>v\<^sub>l\<^sub>h \<sigma>') = must\<langle>[q \<cdot>\<^sub>v\<^sub>i\<^sub>d (\<lambda>x. Action undefined), Cst\<^sub>A undefined]\<rangle>."
@@ -1193,8 +1147,7 @@ qed
 lemma if_must:
   assumes "\<rho> \<Turnstile>\<^sub>l\<^sub>s\<^sub>t ana_pg_fw_must s_BV"
   assumes "\<rho> \<Turnstile>\<^sub>l\<^sub>h must\<langle>[q,d]\<rangle>."
-  shows 
-    "\<rho> \<Turnstile>\<^sub>r\<^sub>h \<^bold>\<not>may[q, d] \<and> \<rho> \<Turnstile>\<^sub>l\<^sub>h anadom\<langle>[d]\<rangle>. \<and> is_Node\<^sub>i\<^sub>d q \<and>is_Elem\<^sub>i\<^sub>d d \<and> the_Elem\<^sub>i\<^sub>d d \<in> analysis_dom"
+  shows "\<rho> \<Turnstile>\<^sub>r\<^sub>h \<^bold>\<not>may[q, d] \<and> \<rho> \<Turnstile>\<^sub>l\<^sub>h anadom\<langle>[d]\<rangle>. \<and> is_Node\<^sub>i\<^sub>d q \<and> is_Elem\<^sub>i\<^sub>d d \<and> the_Elem\<^sub>i\<^sub>d d \<in> analysis_dom"
 proof -
   have Csts: "is_Cst q" "is_Cst d"
     using must_fst_id_is_Cst must_snd_id_is_Cst using assms by auto
@@ -1203,7 +1156,7 @@ proof -
     using solves_lh_least[of ana_pg_fw_must \<rho> s_BV "[q,d]" the_must] fw_may.ana_pg_fw_may_finite
       fw_may.ana_pg_fw_may_stratified by fastforce
 
-  then obtain c where
+  then obtain c where 
     "c \<in> ana_pg_fw_must"
     "lh_consequence \<rho> c (must\<langle>[q,d]\<rangle>.)"
     by auto
@@ -1249,7 +1202,7 @@ qed
 lemma not_must_and_may:
   assumes "[Node q, Elem d] \<in> \<rho> the_must"
   assumes "\<rho> \<Turnstile>\<^sub>l\<^sub>s\<^sub>t ana_pg_fw_must s_BV"
-  assumes "[Node q, Elem d] \<in> \<rho> the_may"                  
+  assumes a: "[Node q, Elem d] \<in> \<rho> the_may"                  
   shows False
 proof -
   have "\<rho> \<Turnstile>\<^sub>l\<^sub>h must\<langle>[Cst\<^sub>N q, Cst\<^sub>E d]\<rangle>."
@@ -1257,7 +1210,7 @@ proof -
   then have "\<rho> \<Turnstile>\<^sub>r\<^sub>h \<^bold>\<not>may [Cst\<^sub>N q, Cst\<^sub>E d]"
     using if_must assms(2) by metis
   then show False
-    using assms(3) by auto
+    using a by auto
 qed
 
 lemma not_solves_must_and_may:
@@ -1332,8 +1285,7 @@ proof -
     by (metis cst.sel(2) assms(1) assms(2) id.sel(2) is_encode_elem_if_must_right_arg)
 
   have not_may: "\<not> \<rho> \<Turnstile>\<^sub>l\<^sub>h may\<langle>[Cst\<^sub>N (end_of \<pi>), d]\<rangle>."
-    using not_solves_must_and_may[OF assms(1), of "(end_of \<pi>)" "the_Elem\<^sub>i\<^sub>d d"] assms(2) \<pi>e d_encdec 
-    by force
+    using not_solves_must_and_may[OF assms(1), of "(end_of \<pi>)" "the_Elem\<^sub>i\<^sub>d d"] assms(2) \<pi>e d_encdec by force
   have "\<not>the_Elem\<^sub>i\<^sub>d d \<in> fw_may.S_hat_path \<pi> (analysis_dom - d_init)"
     using fw_may.sound_ana_pg_fw_may assms(1)
     unfolding fw_may.summarizes_fw_may_def
@@ -1421,8 +1373,7 @@ definition summarizes_bw_must :: "(pred, ('n, 'v, 'd) cst) pred_val \<Rightarrow
          \<rho> \<Turnstile>\<^sub>l\<^sub>h must\<langle>[q, d]\<rangle>. \<longrightarrow>
           (\<forall>\<pi>. \<pi> \<in> path_with_word_from_to (the_Node\<^sub>i\<^sub>d q) end \<longrightarrow> the_Elem\<^sub>i\<^sub>d d \<in> S^\<^sub>P\<lbrakk>\<pi>\<rbrakk> d_init))"
 
-interpretation fw_must: analysis_BV_forward_must 
-  pg_rev analysis_dom "\<lambda>e. (kill_set (rev_edge e))" "(\<lambda>e. gen_set (rev_edge e))" d_init
+interpretation fw_must: analysis_BV_forward_must pg_rev analysis_dom "\<lambda>e. (kill_set (rev_edge e))" "(\<lambda>e. gen_set (rev_edge e))" d_init
   using analysis_BV_forward_must_def finite_pg_rev analysis_BV_backward_must_axioms
     analysis_BV_backward_must_def analysis_BV_backward_must_axioms_def
     analysis_BV_forward_must_axioms.intro finite_program_graph.intro
@@ -1518,21 +1469,12 @@ proof -
   then show ?thesis
     by (metis (no_types, lifting) S_hat_path_forward_backward assms(3) mem_Collect_eq prod.collapse)
 qed
- 
 
 lemma summarizes_bw_must_forward_backward:
   assumes "fw_must.summarizes_fw_must \<rho>"
   shows "summarizes_bw_must \<rho>"
   unfolding summarizes_bw_must_def
-proof(rule; rule ; rule ;rule ;rule)
-  fix q d \<pi>
-  assume "\<rho> \<Turnstile>\<^sub>l\<^sub>h must\<langle>[q, d]\<rangle>."
-  moreover
-  assume "\<pi> \<in> path_with_word_from_to (the_Node\<^sub>i\<^sub>d q) end"
-  ultimately
-  show "the_Elem\<^sub>i\<^sub>d d \<in> S^\<^sub>P\<lbrakk>\<pi>\<rbrakk> d_init"
-    using assms summarizes_fw_must_forward_backward' by auto
-qed
+  using assms summarizes_fw_must_forward_backward' by auto
 
 theorem sound_ana_pg_bw_must:
   assumes "\<rho> \<Turnstile>\<^sub>l\<^sub>s\<^sub>t ana_pg_bw_must s_BV"
